MyPackage/Notation.lean
@@ -4,6 +4,6 @@ import MyPackage.Base
 infix:70 " • " => RSMul.smul
 infix:50 " ∈ " => HasMem.mem
 infixl:60 " ∪ " => HasUnion.union
-infix:50 " ⊂ " => HasIncluded.included -- change to `⊆` ?
+infix:50 " ⊆ " => HasIncluded.included
 infixl:65 " \\ " => HasWithout.without
 notation:max "𝒱 " a:arg => HasVehicle.vehicle a
